theories/Substitution/Introductions/Var.v
@@ -19,4 +19,49 @@ Section Var.
     + epose (eqHead Vσσ'); irrelevance.
   Qed.
   
+  Lemma var0Valid' {Γ l A} (VΓ : [||-v Γ,,A]) (VA : [Γ,,A ||-v<l> A⟨↑⟩ | VΓ]) :
+    [Γ,, A ||-v<l> tRel 0 : _ | VΓ | VA ].
+  Proof.
+    pose proof (invValiditySnoc VΓ) as [? [? [? ]]]; subst.
+    constructor; intros; cbn.
+    + epose (validHead Vσ); irrelevance.
+    + epose (eqHead Vσσ'); irrelevance.
+  Qed.
+
+  Lemma in_ctx_valid {n} :  forall {Γ A} (VΓ : [||-v Γ]), in_ctx Γ n A -> ∑ l, [Γ ||-v<l> A | VΓ].
+  Proof.
+    induction n.
+    - intros ??? h; inversion h; subst.
+      pose proof (invValiditySnoc VΓ) as [? [? [? ]]]; subst.
+      eexists.
+      erewrite <- wk1_ren_on.
+      now eapply wk1ValidTy.
+    - intros ??? h; inversion h; subst.
+      pose proof (invValiditySnoc VΓ) as [? [? [? ]]]; subst.
+      eapply IHn in H13 as [l ?].
+      exists l. erewrite <- wk1_ren_on.
+      now eapply wk1ValidTy.
+  Qed.
+
+  Lemma varnValid {n} :  forall {Γ l A} (VΓ : [||-v Γ]) (h : in_ctx Γ n A) (VA : [Γ ||-v<l> A | VΓ]),
+    [Γ ||-v<l> tRel n : _ | VΓ | VA ].
+  Proof.
+    induction n.
+    - intros ???? h ?; inversion h; subst.
+      eapply var0Valid'.
+    - intros * h ?; inversion h; subst.
+      pose proof (invValiditySnoc VΓ) as [? [VΓ0 [? ]]]; subst.
+      destruct (in_ctx_valid VΓ0 H13).
+      pose proof (h' := H13); eapply IHn, wk1ValidTm in h'; rewrite wk1_ren_on in h'.
+      eapply irrelevanceTm'; tea.
+      now rewrite wk1_ren_on.
+      Unshelve. 1,4: tea.
+  Qed.
+  
+  Lemma var1Valid {Γ l A B} (VΓ : [||-v (Γ,, A) ,, B]) (VA : [_ ||-v<l> A⟨↑⟩⟨↑⟩ | VΓ]) :
+    [(Γ,, A) ,, B ||-v<l> tRel 1 : _ | VΓ | VA ].
+  Proof.
+    eapply varnValid; do 2 constructor.
+  Qed.
+  
 End Var.
