theories/Weakening.v
@@ -387,6 +387,10 @@ Lemma wk_up_ren_subst {Γ Δ Ξ P A n}  (ρ : Γ ≤ Δ) (ρ' : Δ ≤ Ξ) :
   P[n .: ρ ∘w ρ' >> tRel] = P⟨wk_up A ρ'⟩[n .: ρ >> tRel].
 Proof. now bsimpl. Qed.
 
+Lemma shift_subst_scons {B a Γ Δ} (ρ : Δ ≤ Γ) : B⟨↑⟩[a .: ρ >> tRel] = B⟨ρ⟩.
+Proof. bsimpl; now rewrite rinstInst'_term. Qed.
+
+
 Lemma wk_comp_ren_on {Γ Δ Ξ} (H : term) (ρ1 : Γ ≤ Δ) (ρ2 : Δ ≤ Ξ) :
   H⟨ρ2⟩⟨ρ1⟩ = H⟨ρ1 ∘w ρ2⟩.
 Proof. now bsimpl. Qed.
